------------------------------------------------------------------------
-- The equality can be turned into a groupoid which is sometimes
-- commutative
------------------------------------------------------------------------

{-# OPTIONS --cubical-compatible --safe #-}

open import Equality

module Equality.Groupoid
  {reflexive} (eq : ∀ {a p} → Equality-with-J a p reflexive) where

open import Bijection eq using (_↔_)
open Derived-definitions-and-properties eq
open import Equality.Tactic eq
open import Groupoid eq
open import Pointed-type eq
open import Prelude hiding (id; _∘_)

------------------------------------------------------------------------
-- _≡_ comes with a groupoid structure

groupoid : ∀ {a} (A : Type a) → Groupoid a a
groupoid A = record
  { Object = A
  ; _∼_    = _≡_

  ; id  = refl _
  ; _∘_ = flip trans
  ; _⁻¹ = sym

  ; left-identity  = trans-reflʳ
  ; right-identity = trans-reflˡ
  ; assoc          = λ z≡u y≡z x≡y → trans-assoc x≡y y≡z z≡u
  ; left-inverse   = trans-symʳ
  ; right-inverse  = trans-symˡ
  }

------------------------------------------------------------------------
-- In some cases transitivity is commutative

-- This proof is based on an informal proof due to Thierry Coquand,
-- based on a result from homotopy theory.

module Transitivity-commutative
  {a} {A : Type a} (e : A) (_∙_ : A → A → A)
  (left-identity  : ∀ x → (e ∙ x) ≡ x)
  (right-identity : ∀ x → (x ∙ e) ≡ x)
  where

  open Groupoid (groupoid A) hiding (left-identity; right-identity)

  opaque

    commutative : (p q : e ≡ e) → p ∘ q ≡ q ∘ p
    commutative p q =
      p ∘ q                                 ≡⟨ cong (_∘_ p) (lem₁ _) ⟩
      p ∘ (ri ∘ li ⁻¹ ∘ q′ ∘ li ∘ ri ⁻¹)    ≡⟨ prove (Trans (Trans (Trans (Trans (Trans (Sym (Lift ri)) (Lift li)) (Lift q′))
                                                                          (Sym (Lift li))) (Lift ri)) (Lift p))
                                                     (Trans (Trans (Sym (Lift ri))
                                                                              (Trans (Trans (Lift li) (Lift q′)) (Sym (Lift li))))
                                                            (Trans (Lift ri) (Lift p)))
                                                     (refl _) ⟩
      (p ∘ ri) ∘ (li ⁻¹ ∘ q′ ∘ li) ∘ ri ⁻¹  ≡⟨ cong₂ (λ p q → p ∘ q ∘ ri ⁻¹) (lem₂ _) (lem₃ _) ⟩
      (ri ∘ lc p) ∘ rc q′ ∘ ri ⁻¹           ≡⟨ prove (Trans (Trans (Sym (Lift ri)) (Lift (rc q′))) (Trans (Lift (lc p)) (Lift ri)))
                                                     (Trans (Trans (Sym (Lift ri)) (Trans (Lift (rc q′)) (Lift (lc p)))) (Lift ri))
                                                     (refl _) ⟩
      ri ∘ (lc p ∘ rc q′) ∘ ri ⁻¹           ≡⟨ cong (λ p → ri ∘ p ∘ ri ⁻¹) (lem₄ _ _) ⟩
      ri ∘ (rc q′ ∘ lc p) ∘ ri ⁻¹           ≡⟨ prove (Trans (Trans (Sym (Lift ri)) (Trans (Lift (lc p)) (Lift (rc q′)))) (Lift ri))
                                                     (Trans (Trans (Trans (Sym (Lift ri)) (Lift (lc p))) (Lift (rc q′))) (Lift ri))
                                                     (refl _) ⟩
      ri ∘ rc q′ ∘ (lc p ∘ ri ⁻¹)           ≡⟨ cong₂ (λ p q → ri ∘ p ∘ q) (sym (lem₃ _)) (lem₅ _) ⟩
      ri ∘ (li ⁻¹ ∘ q′ ∘ li) ∘ (ri ⁻¹ ∘ p)  ≡⟨ prove (Trans (Trans (Trans (Lift p) (Sym (Lift ri)))
                                                                   (Trans (Trans (Lift li) (Lift q′)) (Sym (Lift li))))
                                                            (Lift ri))
                                                     (Trans (Lift p) (Trans (Trans (Trans (Trans (Sym (Lift ri)) (Lift li)) (Lift q′))
                                                                                   (Sym (Lift li)))
                                                                            (Lift ri)))
                                                     (refl _) ⟩
      (ri ∘ li ⁻¹ ∘ q′ ∘ li ∘ ri ⁻¹) ∘ p    ≡⟨ cong (λ q → q ∘ p) (sym (lem₁ _)) ⟩∎
      q ∘ p                                 ∎
      where

      -- Abbreviations.

      li : ∀ {x} → (e ∙ x) ≡ x
      li = left-identity _

      ri : ∀ {x} → (x ∙ e) ≡ x
      ri = right-identity _

      q′ : e ≡ e
      q′ = li ∘ ri ⁻¹ ∘ q ∘ ri ∘ li ⁻¹

      lc : ∀ {x y} → x ≡ y → (x ∙ e) ≡ (y ∙ e)
      lc = cong (λ x → (x ∙ e))

      rc : ∀ {x y} → x ≡ y → (e ∙ x) ≡ (e ∙ y)
      rc = cong (λ y → (e ∙ y))

      -- Lemmas.

      lem₁ : (p : e ≡ e) →
             p ≡ ri ∘ li ⁻¹ ∘ (li ∘ ri ⁻¹ ∘ p ∘ ri ∘ li ⁻¹) ∘ li ∘ ri ⁻¹
      lem₁ p =
        p                                                          ≡⟨ prove (Lift p) (Trans (Trans Refl (Lift p)) Refl) (refl _) ⟩
        refl _ ∘ p ∘ refl _                                        ≡⟨ sym (cong₂ (λ q r → q ∘ p ∘ r)
                                                                                 (right-inverse _) (right-inverse _)) ⟩
        (ri ∘ ri ⁻¹) ∘ p ∘ (ri ∘ ri ⁻¹)                            ≡⟨ prove (Trans (Trans (Trans (Sym (Lift ri)) (Lift ri)) (Lift p))
                                                                                   (Trans (Sym (Lift ri)) (Lift ri)))
                                                                            (Trans (Trans (Trans (Trans (Trans (Trans
                                                                               (Sym (Lift ri)) Refl) (Lift ri)) (Lift p))
                                                                               (Sym (Lift ri))) Refl) (Lift ri))
                                                                            (refl _) ⟩
        ri ∘ refl _ ∘ ri ⁻¹ ∘ p ∘ ri ∘ refl _ ∘ ri ⁻¹              ≡⟨ sym (cong₂ (λ q r → ri ∘ q ∘ ri ⁻¹ ∘ p ∘ ri ∘ r ∘ ri ⁻¹)
                                                                                 (left-inverse _) (left-inverse _)) ⟩
        ri ∘ (li ⁻¹ ∘ li) ∘ ri ⁻¹ ∘ p ∘ ri ∘ (li ⁻¹ ∘ li) ∘ ri ⁻¹  ≡⟨ prove (Trans (Trans (Trans (Trans (Trans (Trans
                                                                               (Sym (Lift ri)) (Trans (Lift li) (Sym (Lift li))))
                                                                               (Lift ri)) (Lift p)) (Sym (Lift ri)))
                                                                               (Trans (Lift li) (Sym (Lift li)))) (Lift ri))
                                                                            (Trans (Trans (Trans (Trans
                                                                               (Sym (Lift ri)) (Lift li))
                                                                               (Trans (Trans (Trans (Trans
                                                                                  (Sym (Lift li)) (Lift ri)) (Lift p)) (Sym (Lift ri)))
                                                                                  (Lift li))) (Sym (Lift li))) (Lift ri))
                                                                            (refl _) ⟩∎
        ri ∘ li ⁻¹ ∘ (li ∘ ri ⁻¹ ∘ p ∘ ri ∘ li ⁻¹) ∘ li ∘ ri ⁻¹    ∎

      lem₂ : ∀ {x y} (p : x ≡ y) → p ∘ ri ≡ ri ∘ lc p
      lem₂ = elim (λ p → p ∘ ri ≡ ri ∘ lc p) λ _ →
        prove (Trans (Lift ri) Refl)
              (Trans (Cong (λ x → (x ∙ e)) Refl) (Lift ri))
              (refl _)

      lem₃ : ∀ {x y} (p : x ≡ y) → li ⁻¹ ∘ p ∘ li ≡ rc p
      lem₃ = elim (λ p → li ⁻¹ ∘ p ∘ li ≡ rc p) λ x →
        li ⁻¹ ∘ refl x ∘ li  ≡⟨ prove (Trans (Trans (Lift li) Refl) (Sym (Lift li)))
                                      (Trans (Lift li) (Sym (Lift li)))
                                      (refl _) ⟩
        li ⁻¹ ∘ li           ≡⟨ left-inverse _ ⟩
        refl (e ∙ x)         ≡⟨ prove Refl (Cong (λ y → (e ∙ y)) Refl) (refl _) ⟩∎
        rc (refl x)          ∎

      lem₄ : (p q : e ≡ e) → lc p ∘ rc q ≡ rc q ∘ lc p
      lem₄ p q = elim
        (λ {x y} x≡y → lc x≡y ∘ cong (λ z → (x ∙ z)) q ≡
                       cong (λ z → (y ∙ z)) q ∘ lc x≡y)
        (λ x → prove (Trans (Cong (λ z → x ∙ z) (Lift q))
                            (Cong (λ x → x ∙ e) Refl))
                     (Trans (Cong (λ x → x ∙ e) Refl)
                            (Cong (λ z → x ∙ z) (Lift q)))
                     (refl _))
        p

      lem₅ : ∀ {x y} (p : x ≡ y) → lc p ∘ ri ⁻¹ ≡ ri ⁻¹ ∘ p
      lem₅ = elim (λ p → lc p ∘ ri ⁻¹ ≡ ri ⁻¹ ∘ p) λ _ →
        prove (Trans (Sym (Lift ri)) (Cong (λ x → (x ∙ e)) Refl))
              (Trans Refl (Sym (Lift ri)))
              (refl _)

-- In particular, transitivity is commutative for proofs in
-- proj₁ (Ω[ 2 + n ] X).

Ω[2+n]-commutative :
  ∀ {x} {X : Pointed-type x} n →
  (p q : proj₁ (Ω[ 2 + n ] X)) → trans p q ≡ trans q p
Ω[2+n]-commutative {X} n p q =
  Transitivity-commutative.commutative
    id _∘_ left-identity right-identity q p
  where
  open Groupoid (groupoid (proj₁ (Ω[ n ] X)))
